Assignment_2.v
@@ -1,0 +1,1144 @@
+(* Filip Chudy *)
+Require Export Equiv.
+Require Export Hoare2.
+
+(** **** Problem 1 (10 p.) *)
+(** Solve the following exercises: no_whiles (Imp), no_whiles_terminating (Imp).
+*)
+
+Fixpoint no_whiles (c : com) : bool :=
+  match c with
+  | SKIP       => true
+  | _ ::= _    => true
+  | c1 ;; c2  => andb (no_whiles c1) (no_whiles c2)
+  | IFB _ THEN ct ELSE cf FI => andb (no_whiles ct) (no_whiles cf)
+  | WHILE _ DO _ END  => false
+  end.
+
+Inductive no_whilesR: com -> Prop :=
+  | NW_Ass : forall id exp, no_whilesR (id ::= exp)
+  | NW_Seq : forall n m, no_whilesR n -> 
+                         no_whilesR m -> 
+                         no_whilesR (n ;; m)
+  | NW_Skip : no_whilesR SKIP
+  | NW_IfB : forall c1 c2 b, no_whilesR c1 -> 
+                             no_whilesR c2 -> 
+                             no_whilesR (IFB b THEN c1 ELSE c2 FI).
+
+Theorem no_whiles_eqv:
+   forall c, no_whiles c = true <-> no_whilesR c.
+Proof.
+  intros c. split.
+  Case "function -> relation".
+    intros Hfun. induction c; inversion Hfun.
+    SCase "SKIP".
+      apply NW_Skip. 
+    SCase "X ::= a".
+      apply NW_Ass.
+    SCase "c1;; c2".
+      apply andb_true_iff in H0; inversion H0;
+      apply IHc1 in H; apply IHc2 in H1.
+      apply NW_Seq; assumption.
+    SCase "IFB b THEN c1 ELSE c2 FI".
+      apply andb_true_iff in H0; inversion H0;
+      apply IHc1 in H; apply IHc2 in H1.
+      apply NW_IfB; assumption.
+  Case "relation -> function".
+    intros Hrel; induction c; simpl; try reflexivity; inversion Hrel.
+    SCase "c1;; c2".
+      apply IHc1 in H1; apply IHc2 in H2.
+      rewrite H1, H2. reflexivity.
+    SCase "IFB b THEN c1 ELSE c2 END".
+      apply IHc1 in H1. apply IHc2 in H3.
+      rewrite H1, H3. reflexivity.
+Qed.
+
+Theorem no_whiles_terminating : forall c st,
+no_whilesR c -> exists st', c / st || st'.
+Proof.
+  intros c st Hno_whilesR. generalize dependent st.
+  induction c; intros st; inversion Hno_whilesR.
+  Case "SKIP".
+    exists st. apply E_Skip.
+  Case "X ::= a".
+    exists (update st i (aeval st a)). apply E_Ass; reflexivity.
+  Case "c1;; c2".
+    apply IHc1 with st in H1; inversion H1. 
+    apply IHc2 with x in H2; inversion H2.
+    exists x0. apply E_Seq with x; assumption.
+  Case "IFB b THEN c1 ELSE c2 FI".
+    apply IHc1 with st in H1; inversion H1.
+    apply IHc2 with st in H3; inversion H3.
+    remember (beval st b) as evalb. destruct evalb.
+    SCase "b = true".
+      exists x. apply E_IfTrue; try symmetry; assumption.
+    SCase "b = false".
+      exists x0. apply E_IfFalse; try symmetry; assumption.
+Qed.
+
+(** **** Problem 2 (15 p.) *)
+(** Solve the following exercises: break_imp (Imp), 
+                                   while_break_true (Imp), 
+                                   ceval_deterministic (Imp).
+*)
+
+Module BreakImp.
+
+Inductive com : Type :=
+  | CSkip : com
+  | CBreak : com
+  | CAss : id -> aexp -> com
+  | CSeq : com -> com -> com
+  | CIf : bexp -> com -> com -> com
+  | CWhile : bexp -> com -> com.
+
+Tactic Notation "com_cases" tactic(first) ident(c) :=
+  first;
+  [ Case_aux c "SKIP" | Case_aux c "BREAK" 
+  | Case_aux c "::=" | Case_aux c ";"
+  | Case_aux c "IFB" | Case_aux c "WHILE" ].
+
+Notation "'SKIP'" :=
+  CSkip.
+Notation "'BREAK'" :=
+  CBreak.
+Notation "x '::=' a" :=
+  (CAss x a) (at level 60).
+Notation "c1 ; c2" :=
+  (CSeq c1 c2) (at level 80, right associativity).
+Notation "'WHILE' b 'DO' c 'END'" :=
+  (CWhile b c) (at level 80, right associativity).
+Notation "'IFB' c1 'THEN' c2 'ELSE' c3 'FI'" :=
+  (CIf c1 c2 c3) (at level 80, right associativity).
+
+Inductive status : Type :=
+  | SContinue : status
+  | SBreak : status.
+
+Reserved Notation "c1 '/' st '||' s '/' st'"
+                  (at level 40, st, s at level 39).
+
+Inductive ceval : com -> state -> status -> state -> Prop :=
+  | E_Skip : forall st,
+      SKIP / st || SContinue / st
+  | E_Break : forall st,
+      BREAK / st || SBreak / st
+  | E_Ass : forall st id num,
+      (id ::= num) / st || SContinue / (update st id (aeval st num))
+  | E_SeqC : forall c1 c2 st st' st'' sig, c1 / st || SContinue / st' -> 
+              c2 / st' || sig / st'' -> (c1; c2) / st || sig / st''
+  | E_SeqB : forall c1 c2 st st', c1 / st || SBreak / st' -> 
+              (c1; c2) / st || SBreak / st'
+  | E_IfTrue : forall st st' sig c1 c2 b,
+                 beval st b = true -> c1 / st || sig / st' ->
+                 (IFB b THEN c1 ELSE c2 FI) / st || sig / st'
+  | E_IfFalse : forall st st' sig c1 c2 b,
+                 beval st b = false -> c2 / st || sig / st' ->
+                 (IFB b THEN c1 ELSE c2 FI) / st || sig / st'
+  | E_WhileEnd : forall st c b,
+                  beval st b = false -> 
+                  (WHILE b DO c END) / st || SContinue / st
+  | E_WhileLoopC : forall st st' st'' c b,
+                  beval st b = true -> c / st || SContinue / st' ->
+                  (WHILE b DO c END) / st' || SContinue / st'' ->
+                  (WHILE b DO c END) / st || SContinue / st''
+  | E_WhileLoopB : forall st st' c b,
+                  beval st b = true -> c / st || SBreak / st' ->
+                  (WHILE b DO c END) / st || SContinue / st'
+
+  where "c1 '/' st '||' s '/' st'" := (ceval c1 st s st').
+
+Tactic Notation "ceval_cases" tactic(first) ident(c) :=
+  first;
+  [ Case_aux c "E_Skip" | Case_aux c "E_Break" | Case_aux c "E_Ass"
+  | Case_aux c "E_SeqC" | Case_aux c "E_SeqB"
+  | Case_aux c "E_IfTrue" | Case_aux c "E_IfFalse"
+  | Case_aux c "E_WhileEnd"
+  | Case_aux c "E_WhileLoopC"  | Case_aux c "E_WhileLoopB"].
+
+Theorem break_ignore : forall c st st' s,
+     (BREAK; c) / st || s / st' ->
+     st = st'.
+Proof.
+  intros. inversion H. inversion H2. inversion H5. reflexivity.
+Qed.
+
+Theorem while_continue : forall b c st st' s,
+  (WHILE b DO c END) / st || s / st' ->
+  s = SContinue.
+Proof.
+  intros; inversion H; reflexivity.
+Qed.
+
+Theorem while_stops_on_break : forall b c st st',
+  beval st b = true ->
+  c / st || SBreak / st' ->
+  (WHILE b DO c END) / st || SContinue / st'.
+Proof.
+  intros b c st st' Hb Hcb. inversion Hcb;
+    apply E_WhileLoopB; subst; assumption.
+Qed.
+
+Theorem while_break_true : forall b c st st',
+  (WHILE b DO c END) / st || SContinue / st' ->
+  beval st' b = true ->
+  exists st'', c / st'' || SBreak / st'.
+Proof.
+  intros b c st st' Hwhile Hb. remember (WHILE b DO c END) as prog.
+  induction Hwhile; inversion Heqprog; subst.
+  Case "E_WhileEnd".
+    rewrite Hb in H; inversion H.
+  Case "E_WhileLoopC".
+    apply IHHwhile2 in Heqprog; assumption.
+  Case "E_WhileLoopB".
+    exists st. assumption. 
+Qed.
+
+Theorem ceval_deterministic: forall (c:com) st st1 st2 s1 s2,
+     c / st || s1 / st1  ->
+     c / st || s2 / st2 ->
+     st1 = st2 /\ s1 = s2.
+Proof.
+  intros c st st1 st2 s1 s2 Hc1. 
+  generalize dependent s2; generalize dependent st2.
+  induction Hc1; intros st2 s2 Hc2.
+  Case "E_Skip".
+    inversion Hc2; subst; split; try reflexivity.
+  Case "E_Break".
+    inversion Hc2; subst; split; try reflexivity.
+  Case "E_Ass".
+    inversion Hc2; subst; split; try reflexivity.
+  Case "E_SeqC".
+    inversion Hc2; subst.
+    SCase "E_SeqC".
+      apply IHHc1_1 in H1. inversion H1; subst.
+      apply IHHc1_2 in H5. assumption.
+    SCase "E_SeqB".
+      apply IHHc1_1 in H4; inversion H4. inversion H0.
+  Case "E_SeqB".
+    inversion Hc2; subst.
+    SCase "E_SeqC".
+      apply IHHc1 in H1; inversion H1. inversion H0.
+    SCase "E_SeqB".
+      apply IHHc1 in H4. assumption.
+  Case "E_IfTrue".
+    inversion Hc2; subst.
+    SCase "E_IfTrue".
+      apply IHHc1 in H7. assumption.
+    SCase "E_IfFalse".
+      rewrite H6 in H. inversion H.
+  Case "E_IfFalse".
+    inversion Hc2; subst.
+    SCase "E_IfTrue".
+      rewrite H6 in H. inversion H.
+    SCase "E_IfFalse".
+      apply IHHc1 in H7. assumption.
+  Case "E_WhileEnd".
+    inversion Hc2; subst.
+    SCase "E_WhileEnd".
+      split; reflexivity.
+    SCase "E_WhileLoopC".
+      rewrite H2 in H. inversion H.
+    SCase "E_WhileLoopB".
+      rewrite H2 in H. inversion H.
+  Case "E_WhileLoopC".
+    inversion Hc2; subst.
+    SCase "E_WhileEnd".
+      rewrite H5 in H. inversion H.
+    SCase "E_WhileLoopC".
+      apply IHHc1_1 in H3; inversion H3; subst.
+      apply IHHc1_2 in H7. assumption.
+    SCase "E_WhileLoopB".
+      apply IHHc1_1 in H6; inversion H6. inversion H1.
+  Case "E_WhileLoopB".
+    inversion Hc2; subst.
+    SCase "E_WhileEnd".
+      rewrite H5 in H. inversion H.
+    SCase "E_WhileLoopC".
+      apply IHHc1 in H3; inversion H3. inversion H1.
+    SCase "E_WhileLoopB".
+      apply IHHc1 in H6; inversion H6. split; [assumption | reflexivity].       
+Qed.
+
+End BreakImp.
+
+(** **** Problem 3 (20 p.) *)
+(** Solve the following exercises: himp_ceval (Equiv), 
+                                   havoc_swap (Equiv), 
+                                   havoc_copy (Equiv), 
+                                   p1_p2_equiv (Equiv), 
+                                   p_3_p4_equiv (Equiv), 
+                                   p5_p6_equiv (Equiv).  
+*)
+
+Module Himp.
+
+Inductive com : Type :=
+  | CSkip : com
+  | CAss : id -> aexp -> com
+  | CSeq : com -> com -> com
+  | CIf : bexp -> com -> com -> com
+  | CWhile : bexp -> com -> com
+  | CHavoc : id -> com.
+
+Tactic Notation "com_cases" tactic(first) ident(c) :=
+  first;
+  [ Case_aux c "SKIP" | Case_aux c "::=" | Case_aux c ";;"
+  | Case_aux c "IFB" | Case_aux c "WHILE" | Case_aux c "HAVOC" ].
+
+Notation "'SKIP'" :=
+  CSkip.
+Notation "X '::=' a" :=
+  (CAss X a) (at level 60).
+Notation "c1 ;; c2" :=
+  (CSeq c1 c2) (at level 80, right associativity).
+Notation "'WHILE' b 'DO' c 'END'" :=
+  (CWhile b c) (at level 80, right associativity).
+Notation "'IFB' e1 'THEN' e2 'ELSE' e3 'FI'" :=
+  (CIf e1 e2 e3) (at level 80, right associativity).
+Notation "'HAVOC' l" := (CHavoc l) (at level 60).
+
+(** **** Exercise: 2 stars (himp_ceval) *)
+(** Now, we must extend the operational semantics. We have provided
+   a template for the [ceval] relation below, specifying the big-step
+   semantics. What rule(s) must be added to the definition of [ceval]
+   to formalize the behavior of the [HAVOC] command? *)
+
+Reserved Notation "c1 '/' st '||' st'" (at level 40, st at level 39).
+
+Inductive ceval : com -> state -> state -> Prop :=
+  | E_Skip : forall st : state, SKIP / st || st
+  | E_Ass : forall (st : state) (a1 : aexp) (n : nat) (X : id),
+            aeval st a1 = n -> (X ::= a1) / st || update st X n
+  | E_Seq : forall (c1 c2 : com) (st st' st'' : state),
+            c1 / st || st' -> c2 / st' || st'' -> (c1 ;; c2) / st || st''
+  | E_IfTrue : forall (st st' : state) (b1 : bexp) (c1 c2 : com),
+               beval st b1 = true ->
+               c1 / st || st' -> (IFB b1 THEN c1 ELSE c2 FI) / st || st'
+  | E_IfFalse : forall (st st' : state) (b1 : bexp) (c1 c2 : com),
+                beval st b1 = false ->
+                c2 / st || st' -> (IFB b1 THEN c1 ELSE c2 FI) / st || st'
+  | E_WhileEnd : forall (b1 : bexp) (st : state) (c1 : com),
+                 beval st b1 = false -> (WHILE b1 DO c1 END) / st || st
+  | E_WhileLoop : forall (st st' st'' : state) (b1 : bexp) (c1 : com),
+                  beval st b1 = true ->
+                  c1 / st || st' ->
+                  (WHILE b1 DO c1 END) / st' || st'' ->
+                  (WHILE b1 DO c1 END) / st || st''
+  | E_Havoc : forall n X st, (HAVOC X) / st || update st X n
+
+
+  where "c1 '/' st '||' st'" := (ceval c1 st st').
+
+Tactic Notation "ceval_cases" tactic(first) ident(c) :=
+  first;
+  [ Case_aux c "E_Skip" | Case_aux c "E_Ass" | Case_aux c "E_Seq"
+  | Case_aux c "E_IfTrue" | Case_aux c "E_IfFalse"
+  | Case_aux c "E_WhileEnd" | Case_aux c "E_WhileLoop" 
+  | Case_aux c "E_Havoc"
+  ].
+
+Example havoc_example1 : (HAVOC X) / empty_state || update empty_state X 0.
+Proof.
+  apply E_Havoc.
+Qed.
+
+Example havoc_example2 :
+  (SKIP;; HAVOC Z) / empty_state || update empty_state Z 42.
+Proof.
+  apply E_Seq with empty_state. apply E_Skip. apply E_Havoc.
+Qed.
+(** [] *)
+
+Definition cequiv (c1 c2 : com) : Prop := forall st st' : state,
+  c1 / st || st' <-> c2 / st || st'.
+
+(** **** Exercise: 3 stars (havoc_swap) *)
+(** Are the following two programs equivalent? *)
+
+Definition pXY :=
+  HAVOC X;; HAVOC Y.
+
+Definition pYX :=
+  HAVOC Y;; HAVOC X.
+
+(** If you think they are equivalent, prove it. If you think they are
+    not, prove that. *)
+
+Theorem pXY_cequiv_pYX :
+  cequiv pXY pYX \/ ~cequiv pXY pYX.
+Proof.
+  left. (* cequiv pXY pYX *)
+  unfold cequiv, pXY, pYX. intros st st'.
+  assert(Lem: forall A B n1 n2, B <> A ->
+         update (update st B n2) A n1 = update (update st A n1) B n2).
+  Case "proof of Lem".
+    intros A B n1 n2 Hneq. apply functional_extensionality; intros x. 
+    apply update_permute. assumption.
+  split; intros p; inversion p; inversion H1; inversion H4; subst.
+  Case "pXY -> pYX".
+    apply E_Seq with (update st Y n0).
+    SCase "HAVOC Y". 
+      apply E_Havoc.
+    SCase "HAVOC X".
+      rewrite Lem; [apply E_Havoc | intros Hneq; inversion Hneq].
+  Case "pYX -> pXY".
+    apply E_Seq with (update st X n0).
+    SCase "HAVOC X".
+      apply E_Havoc.
+    SCase "HAVOC Y".
+      rewrite Lem; [apply E_Havoc | intros Hneq; inversion Hneq].
+Qed.
+
+(** **** Exercise: 4 stars, optional (havoc_copy) *)
+(** Are the following two programs equivalent? *)
+
+Definition ptwice :=
+  HAVOC X;; HAVOC Y.
+
+Definition pcopy :=
+  HAVOC X;; Y ::= AId X.
+
+(** If you think they are equivalent, then prove it. If you think they
+    are not, then prove that.  (Hint: You may find the [assert] tactic
+    useful.) *)
+
+Theorem ptwice_cequiv_pcopy :
+  cequiv ptwice pcopy \/ ~cequiv ptwice pcopy.
+Proof. 
+  right. (* ~cequiv ptwice pcopy *)
+  unfold cequiv, ptwice, pcopy. intros cont.
+  assert(Htwice: (HAVOC X;; HAVOC Y) / empty_state
+                 || update (update empty_state X 42) Y 1).
+  Case "proof of Htwice".                
+    apply E_Seq with (update empty_state X 42); apply E_Havoc.
+  assert (Hcopy: (HAVOC X;; Y ::= AId X)  / empty_state 
+                 || update (update empty_state X 42) Y 1).
+  Case "proof of Hcopy".
+    apply cont in Htwice. assumption.
+  inversion Hcopy; inversion H1; inversion H4; subst.
+  simpl in H12. rewrite update_eq in H12.
+  remember (beq_nat n 42) as n42; destruct n42.
+  Case "n = 42".
+    apply beq_nat_eq in Heqn42. rewrite Heqn42 in H12.
+    assert(F: update (update empty_state X 42) Y 42 Y
+            = update (update empty_state X 42) Y  1 Y).
+    SCase "proof of false".
+      rewrite H12; reflexivity.
+    rewrite update_eq in F; rewrite update_eq in F; inversion F.
+  Case "n <> 42".
+    assert(F: update (update empty_state X  n) Y n X 
+            = update (update empty_state X 42) Y 1 X).
+    SCase "proof of false".
+      rewrite H12; reflexivity.
+    rewrite update_neq in F; [rewrite update_eq in F | intros HF; inversion HF];
+    rewrite update_neq in F; [rewrite update_eq in F | intros HF; inversion HF].
+    rewrite F in Heqn42; simpl in Heqn42. inversion Heqn42.
+Qed.
+(** [] *)
+
+(** **** Exercise: 5 stars, advanced (p1_p2_equiv) *)
+(** Prove that p1 and p2 are equivalent. In this and the following
+    exercises, try to understand why the [cequiv] definition has the
+    behavior it has on these examples. *)
+
+Definition p1 : com :=
+  WHILE (BNot (BEq (AId X) (ANum 0))) DO
+    HAVOC Y;;
+    X ::= APlus (AId X) (ANum 1)
+  END.
+
+Definition p2 : com :=
+  WHILE (BNot (BEq (AId X) (ANum 0))) DO
+    SKIP
+  END.
+
+
+(** Intuitively, the programs have the same termination
+    behavior: either they loop forever, or they terminate in the
+    same state they started in.  We can capture the termination
+    behavior of p1 and p2 individually with these lemmas: *)
+
+Lemma p1_may_diverge : forall st st', st X <> 0 ->
+  ~ p1 / st || st'.
+Proof.
+  intros st st' H cont; generalize dependent H;
+  remember p1 as p1. induction cont; try inversion Heqp1; subst.
+  Case "E_WhileEnd".
+    simpl in H. apply negb_false_iff in H. apply beq_nat_true in H.
+    intros NotH. contradiction.
+  Case "E_WhileLoop".
+    simpl in H. apply negb_true_iff in H. apply beq_nat_false in H.
+    apply IHcont2 in Heqp1. 
+    SCase "subgoal using IHcont2". 
+      inversion Heqp1.
+    SCase "second condition of IHcont2".
+      inversion cont1; inversion H2; inversion H5; subst. simpl in H5. simpl.
+      rewrite update_eq. rewrite update_neq; [omega | intros HF; inversion HF].
+Qed.
+
+Lemma p2_may_diverge : forall st st', st X <> 0 ->
+  ~ p2 / st || st'.
+Proof.
+  intros st st' H cont; generalize dependent H;
+  remember p2 as p2. induction cont; try inversion Heqp2; subst.
+  Case "E_WhileEnd".
+    simpl in H. apply negb_false_iff in H. apply beq_nat_true in H.
+    intros NotH. contradiction.
+  Case "E_WhileLoop".
+    simpl in H. apply negb_true_iff in H. apply beq_nat_false in H.
+    apply IHcont2 in Heqp2. 
+    SCase "subgoal using IHcont2". 
+      inversion Heqp2.
+    SCase "second condition of IHcont2".
+      inversion cont1; subst. assumption.
+Qed.
+
+(** You should use these lemmas to prove that p1 and p2 are actually
+    equivalent. *)
+
+Theorem p1_p2_equiv : cequiv p1 p2.
+Proof.
+  unfold cequiv, p1, p2. intros st st'. split.
+  Case "p1 -> p2".
+    intros Hp1. inversion Hp1; subst.
+    SCase "E_WhileEnd".
+      apply E_WhileEnd. assumption.
+    SCase "E_WhileLoop".
+      apply E_WhileLoop with st'0; try assumption;
+        simpl in H1; apply negb_true_iff in H1; apply beq_nat_false in H1;
+        apply p1_may_diverge with st st' in H1; contradiction.
+  Case "p2 -> p1".
+    intros Hp2. inversion Hp2; subst.
+    SCase "E_WhileEnd".
+      apply E_WhileEnd. assumption.
+    SCase "E_WhileLoop".
+      apply E_WhileLoop with st'0; try assumption;
+        simpl in H1; apply negb_true_iff in H1; apply beq_nat_false in H1;
+        apply p2_may_diverge with st st' in H1; contradiction.
+Qed.
+
+(** **** Exercise: 4 stars, advanced (p3_p4_inquiv) *)
+
+(** Prove that the following programs are _not_ equivalent. *)
+
+Definition p3 : com :=
+  Z ::= ANum 1;;
+  WHILE (BNot (BEq (AId X) (ANum 0))) DO
+    HAVOC X;;
+    HAVOC Z
+  END.
+
+Definition p4 : com :=
+  X ::= (ANum 0);;
+  Z ::= (ANum 1).
+
+
+Theorem p3_p4_inequiv : ~ cequiv p3 p4.
+Proof.
+  unfold cequiv, p3, p4. intros cont.
+  assert(Hp3: p3 / (update empty_state X 1) 
+              || update (update (update (update empty_state X 1) Z 1) X 0) Z 2).
+  Case "proof of Hp3".
+    apply E_Seq with (update (update empty_state X 1) Z 1).
+    SCase "assignment".
+      apply E_Ass; reflexivity.
+    SCase "while".
+      apply E_WhileLoop with 
+            (update (update (update (update empty_state X 1) Z 1) X 0) Z 2).
+      SSCase "guard".
+        reflexivity.
+      SSCase "body".
+        apply E_Seq with (update (update (update empty_state X 1) Z 1) X 0);
+        apply E_Havoc.
+      SSCase "remaining while".
+        apply E_WhileEnd; reflexivity.
+  apply cont in Hp3. inversion Hp3; subst. inversion H4; subst. simpl in H5.
+  assert(Ext: forall (st st' : state) U, st = st' -> st U = st' U).
+  Case "proof of Ext".
+    intros st st'0 U Heq; rewrite Heq. reflexivity.
+  apply Ext with (U:=Z) in H5. repeat rewrite update_eq in H5. inversion H5.
+Qed.
+
+(** **** Exercise: 5 stars, advanced, optional (p5_p6_equiv) *)
+
+Definition p5 : com :=
+  WHILE (BNot (BEq (AId X) (ANum 1))) DO
+    HAVOC X
+  END.
+
+Definition p6 : com :=
+  X ::= ANum 1.
+
+Lemma p5_stops_with_x_1 : forall st st', 
+  p5 / st || st' -> st' = update st X 1.
+Proof.
+  intros st st' Hp5stops; remember p5 as p5. 
+  ceval_cases (induction Hp5stops) Case; try inversion Heqp5; subst; simpl in H.
+  Case "E_WhileEnd".
+    apply negb_false_iff in H; apply beq_nat_true in H.
+    apply functional_extensionality; intros x.
+    remember (eq_id_dec X x) as sameXx; destruct sameXx.
+    SCase "X = x".
+      rewrite <- e, update_eq. assumption. 
+    SCase "X <> x".
+      rewrite update_neq; [reflexivity | assumption].
+  Case "E_WhileLoop".
+    apply negb_true_iff in H; apply beq_nat_false in H.
+    inversion Hp5stops1; subst.
+    assert(update st X 1 = update (update st X n) X 1).
+    SCase "proof of assertion".
+      apply functional_extensionality; intros x.
+      rewrite update_shadow; reflexivity.
+    apply IHHp5stops2 in Heqp5; rewrite H0. assumption.
+Qed.
+
+
+Theorem p5_p6_equiv : cequiv p5 p6.
+Proof.
+  unfold cequiv, p5, p6. split.
+  Case "p5 -> p6".
+    intros Hp5. apply p5_stops_with_x_1 in Hp5; subst. apply E_Ass; reflexivity.
+  Case "p6 -> p5".
+    intros Hp6. inversion Hp6; subst; simpl.
+    remember (beq_nat (st X) 1) as X1; destruct X1.
+    SCase "st X = 1".
+      apply beq_nat_eq in HeqX1.
+      assert (Hshadow: st = update st X 1).
+      SSCase "proof of Hshadow".
+        apply functional_extensionality. intros x. symmetry; apply update_same.
+        assumption.
+      rewrite <- Hshadow. apply E_WhileEnd. simpl. rewrite HeqX1. reflexivity.
+    SCase "st X <> 1".
+      apply E_WhileLoop with (update st X 1).
+      SSCase "guard".
+        simpl; apply negb_true_iff; symmetry; assumption.
+      SSCase "body".
+        apply E_Havoc.
+      SSCase "remaining iterations".
+        apply E_WhileEnd; reflexivity.
+Qed.
+(** [] *)
+
+End Himp.
+
+(** **** Problem 4 (10 p.) *)
+(** Solve the following exercises: hoare_repeat (Hoare).
+*)
+
+Module RepeatExercise.
+
+(** **** Exercise: 4 stars, advanced (hoare_repeat) *)
+(** In this exercise, we'll add a new command to our language of
+    commands: [REPEAT] c [UNTIL] a [END]. You will write the
+    evaluation rule for [repeat] and add a new Hoare rule to
+    the language for programs involving it. *)
+
+Inductive com : Type :=
+  | CSkip : com
+  | CAsgn : id -> aexp -> com
+  | CSeq : com -> com -> com
+  | CIf : bexp -> com -> com -> com
+  | CWhile : bexp -> com -> com
+  | CRepeat : com -> bexp -> com.
+
+(** [REPEAT] behaves like [WHILE], except that the loop guard is
+    checked _after_ each execution of the body, with the loop
+    repeating as long as the guard stays _false_.  Because of this,
+    the body will always execute at least once. *)
+
+Tactic Notation "com_cases" tactic(first) ident(c) :=
+  first;
+  [ Case_aux c "SKIP" | Case_aux c "::=" | Case_aux c ";"
+  | Case_aux c "IFB" | Case_aux c "WHILE"
+  | Case_aux c "CRepeat" ].
+
+Notation "'SKIP'" := 
+  CSkip.
+Notation "c1 ;; c2" := 
+  (CSeq c1 c2) (at level 80, right associativity).
+Notation "X '::=' a" := 
+  (CAsgn X a) (at level 60).
+Notation "'WHILE' b 'DO' c 'END'" := 
+  (CWhile b c) (at level 80, right associativity).
+Notation "'IFB' e1 'THEN' e2 'ELSE' e3 'FI'" := 
+  (CIf e1 e2 e3) (at level 80, right associativity).
+Notation "'REPEAT' e1 'UNTIL' b2 'END'" := 
+  (CRepeat e1 b2) (at level 80, right associativity).
+
+(** Add new rules for [REPEAT] to [ceval] below.  You can use the rules
+    for [WHILE] as a guide, but remember that the body of a [REPEAT]
+    should always execute at least once, and that the loop ends when
+    the guard becomes true.  Then update the [ceval_cases] tactic to
+    handle these added cases.  *)
+
+Inductive ceval : state -> com -> state -> Prop :=
+  | E_Skip : forall st,
+      ceval st SKIP st
+  | E_Ass  : forall st a1 n X,
+      aeval st a1 = n ->
+      ceval st (X ::= a1) (update st X n)
+  | E_Seq : forall c1 c2 st st' st'',
+      ceval st c1 st' ->
+      ceval st' c2 st'' ->
+      ceval st (c1 ;; c2) st''
+  | E_IfTrue : forall st st' b1 c1 c2,
+      beval st b1 = true ->
+      ceval st c1 st' ->
+      ceval st (IFB b1 THEN c1 ELSE c2 FI) st'
+  | E_IfFalse : forall st st' b1 c1 c2,
+      beval st b1 = false ->
+      ceval st c2 st' ->
+      ceval st (IFB b1 THEN c1 ELSE c2 FI) st'
+  | E_WhileEnd : forall b1 st c1,
+      beval st b1 = false ->
+      ceval st (WHILE b1 DO c1 END) st
+  | E_WhileLoop : forall st st' st'' b1 c1,
+      beval st b1 = true ->
+      ceval st c1 st' ->
+      ceval st' (WHILE b1 DO c1 END) st'' ->
+      ceval st (WHILE b1 DO c1 END) st''
+  | E_RepeatEnd : forall st st' b c,
+      ceval st c st' ->
+      beval st' b = true ->
+      ceval st (REPEAT c UNTIL b END) st'
+  | E_RepeatLoop : forall st st' st'' b c,
+      ceval st c st' ->
+      beval st' b = false ->
+      ceval st' (REPEAT c UNTIL b END) st'' ->
+      ceval st (REPEAT c UNTIL b END) st''
+.
+
+Tactic Notation "ceval_cases" tactic(first) ident(c) :=
+  first;
+  [ Case_aux c "E_Skip" | Case_aux c "E_Ass"
+  | Case_aux c "E_Seq"
+  | Case_aux c "E_IfTrue" | Case_aux c "E_IfFalse"
+  | Case_aux c "E_WhileEnd" | Case_aux c "E_WhileLoop" 
+  | Case_aux c "E_RepeatEnd" | Case_aux c "E_RepeatLoop"
+].
+
+(** A couple of definitions from above, copied here so they use the
+    new [ceval]. *)
+
+Notation "c1 '/' st '||' st'" := (ceval st c1 st') 
+                                 (at level 40, st at level 39).
+
+Definition hoare_triple (P:Assertion) (c:com) (Q:Assertion) 
+                        : Prop :=
+  forall st st', (c / st || st') -> P st -> Q st'.
+
+Notation "{{ P }}  c  {{ Q }}" :=
+  (hoare_triple P c Q) (at level 90, c at next level).
+
+(** To make sure you've got the evaluation rules for [REPEAT] right,
+    prove that [ex1_repeat evaluates correctly. *)
+
+Definition ex1_repeat :=
+  REPEAT
+    X ::= ANum 1;;
+    Y ::= APlus (AId Y) (ANum 1)
+  UNTIL (BEq (AId X) (ANum 1)) END.
+
+Theorem ex1_repeat_works :
+  ex1_repeat / empty_state ||
+               update (update empty_state X 1) Y 1.
+Proof.
+  unfold ex1_repeat. apply E_RepeatEnd.
+    Case "loop body".
+      apply E_Seq with (st':= update empty_state X 1).
+        apply E_Ass; reflexivity.
+        apply E_Ass; reflexivity.
+    Case "loop condition".
+      simpl; reflexivity.
+Qed.
+
+(** Now state and prove a theorem, [hoare_repeat], that expresses an
+    appropriate proof rule for [repeat] commands.  Use [hoare_while]
+    as a model, and try to make your rule as precise as possible. *)
+
+(**
+
+REPEAT c UNTIL b END = c;; WHILE ~b DO c END
+
+
+        ----------------------------------- (hoare_c)
+                    {{P}} c {{Q}}
+
+               {{P /\ b}} c {{P}}
+        -----------------------------------  (hoare_while)
+        {{P}} WHILE b DO c END {{P /\ ~b}}
+
+
+               {{ P }} c1 {{ Q }} 
+               {{ Q }} c2 {{ R }}
+              ---------------------  (hoare_seq)
+              {{ P }} c1;;c2 {{ R }}
+
+ Let b = ~b' and P = P' in hoare_while.
+
+               {{P' /\ ~b'}} c {{P'}}
+        -----------------------------------  (hoare_while)
+        {{P'}} WHILE ~b' DO c END {{P' /\ b'}}
+
+When applied to hoare_seq, we have (with R = P' /\ b', P' = Q).
+
+                                     {{Q /\ ~b'}} c {{Q}}
+                             --------------------------------------
+           {{ P }} c {{ Q }}, {{Q}} WHILE ~b' DO c END {{Q /\ b'}}
+          ----------------------------------------------------------
+                  {{ P }} c;;WHILE ~b' DO c END {{ Q /\ b' }}
+
+which simplifies to
+
+           {{ P }} c {{ Q }}, {{Q /\ ~b'}} c {{Q}}
+          -----------------------------------------
+           {{ P }} REPEAT c UNTIL b' {{ Q /\ b' }}
+
+What's more,
+
+       {{ P }} c {{ Q }}, (Q /\ ~b') ->> P
+    -----------------------------------------
+     {{ P }} c {{ Q }}, {{Q /\ ~b'}} c {{Q}}
+
+So the form of the theorem will be
+
+           {{ P }} c {{ Q }}, (Q /\ ~b') ->> P
+          -----------------------------------------
+           {{ P }} REPEAT c UNTIL b' {{ Q /\ b' }}
+
+We'll use b instead of b'.
+*)
+
+Lemma hoare_repeat : forall P Q b c,
+  {{P}} c {{Q}} ->
+  (fun st => Q st /\ ~(bassn b st)) ->> P ->
+  {{P}} (REPEAT c UNTIL b END) {{fun st => Q st /\ bassn b st}}.
+Proof.
+  intros P Q b c Hc Hbc st st' Hcstates Hp.
+  remember (REPEAT c UNTIL b END) as rcom.
+  ceval_cases (induction Hcstates) Case; 
+  try inversion Heqrcom; subst. 
+  Case "E_RepeatEnd".
+    split.
+    SCase "Q st'".
+      apply Hc in Hcstates; apply Hcstates in Hp. assumption.
+    SCase "bassn b st'".
+      apply bexp_eval_true in H. assumption.
+  Case "E_RepeatLoop".
+    apply IHHcstates2; [reflexivity | apply Hbc].
+    split.
+    SCase "Q st'".
+      apply Hc in Hcstates1; apply Hcstates1 in Hp. assumption.
+    SCase "~ bassn b st'".
+      apply bexp_eval_false in H. assumption.
+Qed.
+
+(* COPYPASTE TO UPDATE HOARE RULES FOR REPEAT...UNTIL *)
+
+Theorem hoare_consequence_post : forall (P Q Q' : Assertion) c,
+  {{P}} c {{Q'}} ->
+  Q' ->> Q ->
+  {{P}} c {{Q}}.
+Proof.
+  intros P Q Q' c Hhoare Himp.
+  intros st st' Hc HP.
+  apply Himp.
+  apply (Hhoare st st').
+  assumption. assumption. Qed.
+
+Theorem hoare_seq : forall P Q R c1 c2,
+  {{Q}} c2 {{R}} ->
+  {{P}} c1 {{Q}} ->
+  {{P}} c1;;c2 {{R}}.
+Proof.
+  intros P Q R c1 c2 H1 H2 st st' H12 Pre.
+  inversion H12; subst.
+  apply (H1 st'0 st'); try assumption.
+  apply (H2 st st'0); assumption. Qed.
+
+Theorem hoare_consequence_pre : forall (P P' Q : Assertion) c,
+  {{P'}} c {{Q}} ->
+  P ->> P' ->
+  {{P}} c {{Q}}.
+Proof.
+  intros P P' Q c Hhoare Himp.
+  intros st st' Hc HP. apply (Hhoare st st').
+  assumption. apply Himp. assumption. Qed.
+
+Theorem hoare_asgn : forall Q X a,
+{{assn_sub X a Q}} (X ::= a) {{Q}}.
+Proof.
+  unfold hoare_triple.
+  intros Q X a st st' HE HQ.
+  inversion HE. subst.
+  unfold assn_sub in HQ. assumption. Qed.
+
+(* COPYPASTE ENDS *)
+
+Theorem hoare_repeat_works:
+  {{ fun st => st X > 0 }}
+  REPEAT
+    Y ::= AId X;;
+    X ::= AMinus (AId X) (ANum 1)
+  UNTIL BEq (AId X) (ANum 0) END
+  {{ fun st => st X = 0 /\ st Y > 0 }}.
+Proof.
+  remember (fun st => st Y > 0) as Q.
+  remember (BEq (AId X) (ANum 0)) as b.
+  remember (Y ::= AId X;;
+            X ::= AMinus (AId X) (ANum 1)) as c.
+  remember (REPEAT c UNTIL b END) as prog.
+  assert((fun st => Q st /\ bassn b st) ->> (fun st => st X = 0 /\ st Y > 0)).
+  Case "proof of assertion".
+    intros st. rewrite HeqQ, Heqb; unfold bassn; simpl.
+    intros Hs; inversion Hs. split; 
+    [apply beq_nat_true; assumption | assumption].
+  apply hoare_consequence_post with
+        (P:=(fun st => st X > 0))
+        (Q:=(fun st : state => st X = 0 /\ st Y > 0))
+        (Q':=(fun st : state => Q st /\ bassn b st))
+        (c:=prog).
+  rewrite Heqprog, Heqc. apply hoare_repeat.
+  Case "loop body".
+    apply hoare_seq with Q;
+    eapply hoare_consequence_pre;
+    [ apply hoare_asgn | rewrite HeqQ; intros st HQ; unfold assn_sub; simpl
+    | apply hoare_asgn | rewrite HeqQ; intros st HQ; unfold assn_sub; simpl];
+    [ rewrite update_neq; [assumption | intros HF; inversion HF]
+    | rewrite update_eq; assumption].
+  Case "assertion convertion".
+    rewrite HeqQ,Heqb; unfold bassn; simpl; intros st Qb. inversion Qb.
+    apply not_true_is_false in H1.
+    destruct (st X); [inversion H1 | omega].
+  Case "another assertion convertion".
+    rewrite HeqQ,Heqb; unfold bassn; simpl; intros st Qb. inversion Qb.
+    apply beq_nat_true in H1. split; assumption.
+Qed.
+
+End RepeatExercise.
+
+(** **** Problem 5 (5 p.) *)
+(** Solve the following exercises: add_slowly_decoration (Hoare2).
+*)
+
+(** **** Exercise: 3 stars, optional (add_slowly_decoration) *)
+(** The following program adds the variable X into the variable Z
+    by repeatedly decrementing X and incrementing Z.
+  WHILE X <> 0 DO
+     Z ::= Z + 1;
+     X ::= X - 1
+  END
+
+    Following the pattern of the [subtract_slowly] example above, pick
+    a precondition and postcondition that give an appropriate
+    specification of [add_slowly]; then (informally) decorate the
+    program accordingly. *)
+(*
+(1) {{ X = n /\ Z = m }} ->>
+(2) {{ Z + X = m + n }}
+  WHILE X <> 0 DO
+(3) {{ Z + X = m + n /\ X <> 0 }} ->>
+(4) {{ (Z + 1) + (X - 1) = m + n }}
+     Z ::= Z + 1;
+(5) {{ Z + (X - 1) = m + n }}
+     X ::= X - 1
+(6) {{ Z + X = m + n }}
+  END
+(7) {{ Z + X = m + n /\ ~(X <> 0) }} ->>
+(8) {{ Z = m + n }}
+*)
+
+Theorem add_slowly_correct : forall n m,
+    {{ fun st => st X = n /\ st Z = m }}
+  WHILE BNot (BEq (AId X) (ANum 0)) DO
+    Z ::= APlus (AId Z) (ANum 1);;
+    X ::= AMinus (AId X) (ANum 1)
+  END
+    {{ fun st => st Z = m + n }}.
+Proof.
+  intros n m.
+  eapply hoare_consequence_post.
+  Case "(1)..(7)".
+    apply hoare_consequence_pre with (fun st => (st X) + (st Z) = m + n).
+    SCase "(2)..(7)".
+      apply hoare_while. eapply hoare_consequence_pre.
+      SSCase "(4)..(6)".
+        eapply hoare_seq; apply hoare_asgn.
+      SSCase "(3) ->> (4)".
+        intros st [Hst Hb]. unfold assn_sub. simpl. rewrite update_eq.
+        rewrite <- Hst. rewrite update_neq. rewrite update_neq.
+        rewrite update_eq, plus_assoc. 
+        unfold bassn in Hb; simpl in Hb; apply negb_true_iff in Hb.
+        destruct (st X).
+        SSSCase "st X = 0". 
+          inversion Hb.
+        SSSCase "st X <> 0".
+          simpl. omega.
+        intros HF; inversion HF.
+        intros HF; inversion HF.
+    SCase "(1) ->> (2)".
+      intros st [H0 H1]. rewrite H0, H1. omega.
+  Case "(7) ->> (8)".
+    intros st [Hst Hb]. rewrite <- Hst. unfold bassn in Hb; simpl in Hb. 
+    apply not_true_is_false in Hb. apply negb_false_iff in Hb. 
+    apply beq_nat_true in Hb. rewrite Hb; reflexivity.
+Qed.
+
+
+(** **** Problem 6 (5 p.) *)
+(** Solve the following exercises: parity_formal (Hoare2).
+*)
+
+(** **** Exercise: 3 stars, optional (parity_formal) *)
+(** Translate this proof to Coq. Refer to the reduce-to-zero example
+    for ideas. You may find the following two lemmas useful: *)
+
+Lemma parity_ge_2 : forall x,
+  2 <= x ->
+  parity (x - 2) = parity x.
+Proof.
+  induction x; intro. reflexivity.
+  destruct x. inversion H. inversion H1.
+  simpl. rewrite <- minus_n_O. reflexivity.
+Qed.
+
+Lemma parity_lt_2 : forall x,
+  ~ 2 <= x ->
+  parity (x) = x.
+Proof.
+  intros. induction x. reflexivity. destruct x. reflexivity.
+    apply ex_falso_quodlibet. apply H. omega.
+Qed.
+
+(*
+  (1)    {{ X = m }} ->>                              (a - OK)
+  (2)    {{ parity X = parity m }}
+    WHILE 2 <= X DO
+  (3)      {{ parity X = parity m /\ 2 <= X }}  ->>    (c - OK)
+  (4)      {{ parity (X-2) = parity m }}
+  (5)    X ::= X - 2
+  (6)      {{ parity X = parity m }}
+    END
+  (7)    {{ parity X = parity m /\ X < 2 }}  ->>       (b - OK)
+  (8)    {{ X = parity m }}
+*)
+
+Theorem parity_correct : forall m,
+    {{ fun st => st X = m }}
+  WHILE BLe (ANum 2) (AId X) DO
+    X ::= AMinus (AId X) (ANum 2)
+  END
+    {{ fun st => st X = parity m }}.
+Proof.
+  intros m.
+  eapply hoare_consequence_post.
+  Case "(1)..(7)".
+    apply hoare_consequence_pre with (fun st => parity (st X) = parity m).
+    SCase "(2)..(7)".
+      apply hoare_while. eapply hoare_consequence_pre.
+      SSCase "(4)..(6)".
+        apply hoare_asgn.
+      SSCase "(3) ->> (4)".
+        intros st [Hst Hb]. unfold assn_sub. simpl. rewrite update_eq.
+        rewrite <- Hst. apply parity_ge_2. unfold bassn in Hb. simpl in Hb.
+        destruct (st X) as [|x']; try inversion Hb. 
+        destruct x' as [|x'']; try inversion Hb. omega.
+    SCase "(1) ->> (2)".
+      intros st H. rewrite H. reflexivity.
+  Case "(7) ->> (8)".
+    intros st [Hst Hb]. rewrite <- Hst. unfold bassn in Hb; simpl in Hb. 
+    apply not_true_is_false in Hb.
+    destruct (st X) as [|x']; try reflexivity. 
+    destruct x' as [|x'']; try reflexivity. inversion Hb.
+Qed.
+
+(** **** Problem 7 (5 p.) *)
+(** Solve the following exercises: factorial_dec (Hoare2).
+*)
+
+(** **** Exercise: 4 stars, advanced (factorial_dec)  *)
+(** Remember the factorial function we worked with before: *)
+
+Fixpoint real_fact (n:nat) : nat :=
+  match n with
+  | O => 1
+  | S n' => n * (real_fact n')
+  end.
+
+(** Following the pattern of [subtract_slowly_dec], write a decorated
+    program that implements the factorial function and prove it
+    correct. *)
+
+(*
+  (1) {{ X = n }}
+      ->>
+  (2) {{ 1 * (real_fact X) = real_fact n }}
+  Y ::= 1;;
+  (3) {{ Y * (real_fact X) = real_fact n }}
+  WHILE X <> 0 DO
+  (4) {{ Y * (real_fact X) = real_fact n /\ X >= 0 }}
+      ->>
+  (5) {{ (Y * X) * (real_fact (X - 1)) = real_fact n }}
+    Y ::= Y * X;;
+  (6) {{ Y * (real_fact (X - 1)) = real_fact n }}
+    X ::= X - 1
+  (7) {{ Y * (real_fact X) = real_fact n }}
+  END
+  (8) {{ Y * (real_fact X) = real_fact n /\ ~(X >= 0) }}
+      ->>
+  (9) {{ Y = real_fact n }}
+*)
+
+Theorem factorial_dec: forall n,
+  {{ fun st => st X = n }}
+  Y ::= ANum 1;;
+  WHILE BNot (BEq (AId X) (ANum 0)) DO
+    Y ::= AMult (AId Y) (AId X);;
+    X ::= AMinus (AId X) (ANum 1)
+  END
+  {{ fun st => st Y = real_fact n }}.
+Proof.
+  intros n.
+  eapply hoare_consequence_post.
+  Case "(1)..(8)".
+   eapply hoare_consequence_pre. 
+   SCase "(2)..(8)".
+     apply hoare_seq with
+           (fun st => st Y * real_fact (st X) = real_fact n).
+     SSCase "(3)..(8)".
+       apply hoare_while. eapply hoare_consequence_pre.
+       SSSCase "(5)..(7)".
+         eapply hoare_seq.
+         SSSSCase "(6)..(7)".
+           apply hoare_asgn.
+         SSSSCase "(5)..(6)".
+           apply hoare_asgn.
+       SSSCase "(4) ->> (5)".
+         intros st [Hst Hb]. unfold assn_sub. simpl.
+         rewrite update_eq. rewrite update_neq; 
+         try intros HNeq; try inversion HNeq.
+         rewrite update_eq. rewrite update_neq; 
+         try intros HNeq; try inversion HNeq. 
+         unfold bassn in Hb. simpl in Hb.
+         destruct (st X).
+         SSSSCase "st X = 0".
+           simpl in Hb. inversion Hb.
+         SSSSCase "st X > 0". 
+           unfold real_fact in Hst. fold real_fact in Hst. rewrite <- Hst.
+           assert(S n0 - 1 = n0). omega.
+           rewrite H. rewrite mult_assoc. omega.
+     SSCase "(2)..(3)".
+       apply hoare_asgn.
+   SCase "(1) ->> (2)".
+     intros st Hst. unfold assn_sub. rewrite update_eq.
+     rewrite update_neq; try intros HNeq; try inversion HNeq.
+     simpl. rewrite Hst. omega.
+  Case "(8) ->> (9)".
+    intros st [Hst Hb]. unfold bassn in Hb. apply not_true_is_false in Hb.
+    simpl in Hb. destruct (st X) as [|x']. 
+    SCase "st X = 0".
+      simpl in Hst. rewrite <- Hst. omega.
+    SCase "st X > 0".
+      simpl in Hb. inversion Hb.
+Qed.
